# Hyperbolic

## Hyperbolic Functions

$$
sinh(x)=\frac{e^{x}-e^{-x}}{2}
$$

$$
cosh(x)=\frac{e^{x}+e^{-x}}{2}
$$

$$
tanh(x)=\frac{sinh(x)}{cosh(x)}
$$

$$
csch(x)=\frac{1}{sinh(x)}
$$

$$
sech(x)=\frac{1}{cosh(x)}
$$

$$
coth(x)=\frac{cosh(x)}{sinh(x)}
$$

## Hyperbolic Identities

$$
sinh(-x)=-sinh(x)
$$

$$
cosh(-x)=cosh(x)
$$

$$
cosh^{2}(x)-sinh^{2}(x)=1
$$

$$
1-tanh^{2}(x)=sech^{2}(x)
$$

$$
sinh(x+y)=sinh(x)cosh(y)+cosh(x)sinh(y)
$$

$$
cosh(x+y)=cosh(x)cosh(y)+sinh(x)sinh(y)
$$

## Derivatives of Hyperbolic Functions

$$
\frac{d}{dx}(sinh(x))=cosh(x)
$$

$$
\frac{d}{dx}(cosh(x))=sinh(x)
$$

$$
\frac{d}{dx}(tanh(x))=sech^{2}(x)
$$

$$
\frac{d}{dx}(csch(x))=-csch(x)coth(x)
$$

$$
\frac{d}{dx}(sech(x))=-sech(x)tanh(x)
$$

$$
\frac{d}{dx}(coth(x))=-csch^{2}(x)
$$

## Inverse of Hyperbolic Functions

$$
sinh^{-1}(x)=ln(x+\sqrt{x^{2}+1})\quad x\in\mathbf{R}
$$

$$
cosh^{-1}(x)=ln(x+\sqrt{x^{2}-1})\quad x\geq1
$$

$$
tanh^{-1}(x)=\frac{1}{2}ln\biggl(\frac{1+x}{1-x}\biggr)\quad-1<x<1
$$

$$
csch^{-1}(x)=ln\biggl(\frac{1}{x}+\sqrt{\frac{1}{x^{2}}+1}\biggr)\quad x\in\mathbf{R},\ x\neq 0
$$

$$
sech^{-1}(x)=ln\biggl(\frac{1}{x}+\sqrt{\frac{1}{x^{2}}-1}\biggr)\quad 0<x\leq 1
$$

$$
coth^{-1}(x)=\frac{1}{2}ln\biggl(\frac{x+1}{x-1}\biggr)\quad x<-1\ or\ x>1
$$

## Derivatives of Hypberbolic Functions

$$
\frac{d}{dx}(sinh^{-1}(x))=\frac{1}{\sqrt{x^{2}+1}}\quad x\in\mathbf{R}
$$

$$
\frac{d}{dx}(cosh^{-1}(x))=\frac{1}{\sqrt{x^{2}-1}}\quad x>1
$$

$$
\frac{d}{dx}(tanh^{-1}(x))=\frac{1}{1-x^{2}}\quad-1<x<1
$$

$$
\frac{d}{dx}(csch^{-1}(x))=-\frac{1}{\lvert x \rvert\sqrt{1+x^{2}}}\quad x\in\mathbf{R},\ x\neq 0
$$

$$
\frac{d}{dx}(sech^{-1}(x))=-\frac{1}{x\sqrt{1-x^{2}}}\quad 0<x\leq 1
$$

$$
\frac{d}{dx}(coth^{-1}(x))=\frac{1}{1-x^{2}}\quad x<-1\ or\ x>1
$$