# Trigonometry

## Trigonometric Identities

### Reciprocal Identities

$$
csc(x)=\frac{1}{sin(x)}
$$

$$
sec(x)=\frac{1}{cos(x)}
$$

$$
cot(x)=\frac{1}{tan(x)}
$$

### Quotient Identities

$$
tan(x)=\frac{sin(x)}{cos(x)}
$$

$$
cot(x)=\frac{cos(x)}{sin(x)}
$$

### Pythagorean Identities

$$
sin^{2}(x)+cos^{2}(x)=1
$$

$$
1+tan^{2}(x)=sec^{2}(x)
$$

$$
1+cot^{2}(x)=csc^{2}(x)
$$

### Angle Sum and Difference Identities

$$
sin(x \pm y)=sin(x)cos(y) \pm cos(x)sin(y)
$$

$$
cos(x \pm y)=cos(x)cos(y) \mp sin(x)sin(y)
$$

$$
tan(x \pm y)=\frac{tan(x) \pm tan(y)}{1 \mp tan(x)tan(y)}
$$

$$
csc(x \pm y)=\frac{sec(x)sec(y)csc(x)csc(y)}{sec(x)csc(y) \pm csc(x)sec(y)}$$

$$
sec(x \pm y)=\frac{sec(x)sec(y)csc(x)csc(y)}{csc(x)csc(y) \mp sec(x)sec(y)}
$$

$$
cot(x \pm y) = \frac{cot(x)cot(y) \mp 1}{cot(x) \pm cot(y)}
$$

### Double Angle Identities

$$
sin(2x)=2sin(x)cos(x)
$$

$$
cos(2x)=cos^{2}(x)-sin^{2}(x)=2cos^{2}(x)-1=1-2sin^{2}(x)
$$

$$
tan(2x)=\frac{2tan(x)}{1-tan^{2}(x)}
$$

### Half Angle Identities

$$
sin\biggl(\frac{x}{2}\biggr)=\pm\sqrt{\frac{1-cos(x)}{2}}
$$

$$
cos\biggl(\frac{x}{2}\biggr)=\pm\sqrt{\frac{1+cos(x)}{2}}
$$

$$
tan\biggl(\frac{x}{2}\biggr)=\pm\sqrt{\frac{1-cos(x)}{1+cos(x)}}=\frac{1-cos(x)}{sin(x)}=\frac{sin(x)}{1+cos(x)}
$$

### Squared Identities

$$
sin^{2}(x)=\frac{1-cos(2x)}{2}
$$

$$
cos^{2}(x)=\frac{1+cos(2x)}{2}
$$

$$
tan^{2}(x)=\frac{1-cos(2x)}{1+cos(2x)}
$$

$$
csc^{2}(x)=\frac{2}{1-cos(2x)}
$$

$$
sec^{2}(x)=\frac{2}{1+cos(2x)}
$$

$$
cot^{2}(x)=\frac{1+cos(2x)}{1-cos(2x)}
$$

### Product Identities

$$
cos(x)cos(y)=\frac{1}{2}\bigl(cos(x-y)+cos(x+y)\bigr)
$$

$$
sin(x)sin(y)=\frac{1}{2}\bigl(cos(x-y)-cos(x+y)\bigr)
$$

$$
sin(x)cos(y)=\frac{1}{2}\bigl(sin(x+y)+sin(x-y)\bigr)
$$

$$
cos(x)sin(y)=\frac{1}{2}\bigl(sin(x+y)-sin(x-y)\bigr)
$$

### Sum and Difference Identities

$$
sin(x)+sin(y)=2sin(\frac{x+y}{2})cos(\frac{x-y}{2})
$$

$$
sin(x)-sin(y)=2sin(\frac{x-y}{2})cos(\frac{x+y}{2})
$$

$$
cos(x)+cos(y)=2cos(\frac{x+y}{2})cos(\frac{x-y}{2})
$$

$$
cos(x)-cos(y)=-2sin(\frac{x+y}{2})sin(\frac{x-y}{2})
$$

$$
tan(x)+tan(y)=\frac{sin(x+y)}{cos(x)cos(y)}
$$

$$
tan(x)-tan(y)=\frac{sin(x-y)}{cos(x)cos(y)}
$$

## Derivatives of Trigonometric Functions

$$
\frac{d}{dx}(sin(x))=cos(x)
$$

$$
\frac{d}{dx}(cos(x))=-sin(x)
$$

$$
\frac{d}{dx}(tan(x))=sec^{2}(x)
$$

$$
\frac{d}{dx}(csc(x))=-csc(x)cot(x)
$$

$$
\frac{d}{dx}(sec(x))=sec(x)tan(x)
$$

$$
\frac{d}{dx}(cot(x))=-csc^{2}(x)
$$

## Derivatives of Inverse Trigonometric Functions

$$
\frac{d}{dx}(sin^{-1}(x))=\frac{1}{\sqrt{1-x^{2}}}
$$

$$
\frac{d}{dx}(cos^{-1}(x))=-\frac{1}{\sqrt{1-x^{2}}}
$$

$$
\frac{d}{dx}(tan^{-1}(x))=\frac{1}{1+x^{2}}
$$

$$
\frac{d}{dx}(csc^{-1}(x))=-\frac{1}{x\sqrt{x^{2}-1}}
$$

$$
\frac{d}{dx}(sec^{-1}(x))=\frac{1}{x\sqrt{x^{2}-1}}
$$

$$
\frac{d}{dx}(tan^{-1}(x))=-\frac{1}{1+x^{2}}
$$

## Limits of Trigonometric Functions

$$
\underset{{x\rightarrow 0}}{lim}\frac{sin(x)}{x}=1
$$

$$
\underset{{x\rightarrow 0}}{lim}\frac{cos(x)-1}{x}=0
$$